examples/dsls/mini_steel/Pulse.Typing.fst
@@ -16,47 +16,47 @@ module FTB = FStar.Tactics
 //     ///\ star etc
 //   }
 
-let tm_unit : pure_term = Tm_FVar unit_lid
-let tm_bool : pure_term = Tm_FVar bool_lid
-let tm_true : pure_term = Tm_Constant (Bool true)
-let tm_false : pure_term = Tm_Constant (Bool false)
+let tm_unit = Tm_FVar unit_lid
+let tm_bool = Tm_FVar bool_lid
+let tm_true = Tm_Constant (Bool true)
+let tm_false = Tm_Constant (Bool false)
 
-let mk_erased (u:universe) (t:pure_term) : pure_term =
+let mk_erased (u:universe) (t:term) : term =
   let hd = Tm_UInst erased_lid [u] in
   Tm_PureApp hd None t
 
-let mk_reveal (u:universe) (t:pure_term) (e:pure_term) : pure_term =
+let mk_reveal (u:universe) (t:term) (e:term) : term =
   let hd = Tm_UInst reveal_lid [u] in
   let hd = Tm_PureApp hd (Some Implicit) t in
   Tm_PureApp hd None e
 
 let mk_eq2 (u:universe)
-           (t:pure_term)
-           (e0 e1:pure_term) 
-  : pure_term
+           (t:term)
+           (e0 e1:term) 
+  : term
   = Tm_PureApp
          (Tm_PureApp (Tm_PureApp (Tm_UInst R.eq2_qn [u]) (Some Implicit) t)
                      None e0) None e1
 
-let mk_vprop_eq (e0 e1:pure_term) : pure_term =
+let mk_vprop_eq (e0 e1:term) : term =
   mk_eq2 (U_succ (U_succ U_zero)) Tm_VProp e0 e1
 
-let return_comp (u:universe) (t:pure_term) (e:pure_term)
-  : pure_comp 
+let return_comp (u:universe) (t:term) (e:term)
+  : comp 
   = C_ST { u;
            res = t;
            pre = Tm_Emp;
            post = Tm_Pure (mk_eq2 u t (null_bvar 0) e) }
 
-let return_comp_noeq (u:universe) (t:pure_term)
-  : pure_comp 
+let return_comp_noeq (u:universe) (t:term)
+  : comp 
   = C_ST { u;
            res = t;
            pre = Tm_Emp;
            post = Tm_Emp }
 
-let eqn = pure_term & pure_term & pure_term
-let binding = either pure_term eqn
+let eqn = term & term & term
+let binding = either term eqn
 let env = list (var & binding)
 
 //
@@ -68,15 +68,15 @@ let env = list (var & binding)
 let elab_eqn (e:eqn)
   : R.term
   = let ty, l, r = e in
-    let ty = elab_pure ty in
-    let l = elab_pure l in
-    let r = elab_pure r in
+    let ty = elab_term ty in
+    let l = elab_term l in
+    let r = elab_term r in
     RT.eq2 (R.pack_universe R.Uv_Zero) ty l r
 
 let elab_binding (b:binding)
   : R.term 
   = match b with
-    | Inl t -> elab_pure t
+    | Inl t -> elab_term t
     | Inr eqn -> elab_eqn eqn
 
 module L = FStar.List.Tot
@@ -95,7 +95,7 @@ let rec lookup (e:list (var & 'a)) (x:var)
     | (y, v) :: tl -> if x = y then Some v else lookup tl x
 
 let lookup_ty (e:env) (x:var)
-  : option pure_term
+  : option term
   = match lookup e x with
     | Some (Inl t) -> Some t
     | _ -> None
@@ -145,432 +145,245 @@ let fresh_is_fresh (e:env)
 
 [@@ erasable; no_auto_projectors]
 noeq
-type vprop_equiv (f:RT.fstar_top_env) : env -> pure_term -> pure_term -> Type =
+type vprop_equiv (f:RT.fstar_top_env) : env -> term -> term -> Type =
   | VE_Refl:
      g:env ->
-     t:pure_term ->
+     t:term ->
      vprop_equiv f g t t
 
   | VE_Sym:
      g:env ->
-     t1:pure_term -> 
-     t2:pure_term -> 
+     t1:term -> 
+     t2:term -> 
      vprop_equiv f g t1 t2 ->
      vprop_equiv f g t2 t1
 
   | VE_Trans:
      g:env ->
-     t0:pure_term ->
-     t1:pure_term ->
-     t2:pure_term ->
+     t0:term ->
+     t1:term ->
+     t2:term ->
      vprop_equiv f g t0 t1 ->
      vprop_equiv f g t1 t2 ->
      vprop_equiv f g t0 t2
 
   | VE_Ctxt:
      g:env ->
-     t0:pure_term -> 
-     t1:pure_term -> 
-     t0':pure_term -> 
-     t1':pure_term ->
+     t0:term -> 
+     t1:term -> 
+     t0':term -> 
+     t1':term ->
      vprop_equiv f g t0 t0' ->
      vprop_equiv f g t1 t1' ->
      vprop_equiv f g (Tm_Star t0 t1) (Tm_Star t0' t1')
      
   | VE_Unit: (*   *)
      g:env ->
-     t:pure_term ->
+     t:term ->
      vprop_equiv f g (Tm_Star Tm_Emp t) t
 
   | VE_Comm:
      g:env ->
-     t0:pure_term ->
-     t1:pure_term ->
+     t0:term ->
+     t1:term ->
      vprop_equiv f g (Tm_Star t0 t1) (Tm_Star t1 t0)
      
   | VE_Assoc:
      g:env ->
-     t0:pure_term ->
-     t1:pure_term ->
-     t2:pure_term ->
+     t0:term ->
+     t1:term ->
+     t2:term ->
      vprop_equiv f g (Tm_Star t0 (Tm_Star t1 t2)) (Tm_Star (Tm_Star t0 t1) t2)
 
   | VE_Ext:
      g:env ->
-     t0:pure_term ->
-     t1:pure_term ->
-     FTB.prop_validity_token (extend_env_l f g) (elab_pure (mk_vprop_eq t0 t1)) ->
+     t0:term ->
+     t1:term ->
+     FTB.prop_validity_token (extend_env_l f g) (elab_term (mk_vprop_eq t0 t1)) ->
      vprop_equiv f g t0 t1
 
   // | VE_Ex:
   //    g:env ->
   //    x:var { None? (lookup_ty g x) } ->
-  //    ty:pure_term ->
-  //    t0:pure_term ->
-  //    t1:pure_term ->
+  //    ty:term ->
+  //    t0:term ->
+  //    t1:term ->
   //    vprop_equiv f ((x, Inl ty)::g) (open_term t0 x) (open_term t1 x) ->
   //    vprop_equiv f g (Tm_ExistsSL ty t0) (Tm_ExistsSL ty t1)
 
   // | VE_Fa:
   //    g:env ->
   //    x:var { None? (lookup_ty g x) } ->
-  //    ty:pure_term ->
-  //    t0:pure_term ->
-  //    t1:pure_term ->
+  //    ty:term ->
+  //    t0:term ->
+  //    t1:term ->
   //    vprop_equiv f ((x, Inl ty)::g) (open_term t0 x) (open_term t1 x) ->
   //    vprop_equiv f g (Tm_ForallSL ty t0) (Tm_ForallSL ty t1)
 
 
-let add_frame (s:pure_comp_st) (frame:pure_term)
-  : pure_comp_st =
-
-  let add_frame_s (s:st_comp { is_pure_st_comp s }) : x:st_comp { is_pure_st_comp x } =
-    { s with pre = Tm_Star s.pre frame;
-             post = Tm_Star s.post frame } in
-  match s with
-  | C_ST s -> C_ST (add_frame_s s)
-  | C_STAtomic inames s -> C_STAtomic inames (add_frame_s s)
-  | C_STGhost inames s -> C_STGhost inames (add_frame_s s)
-
-let close_pure_comp (c:pure_comp) (x:var) : pure_comp = close_comp c x
+let add_frame (s:comp_st) (frame:term)
+  : comp_st
+  = let add_frame_s (s:st_comp) : x:st_comp =
+        { s with pre = Tm_Star s.pre frame;
+                 post = Tm_Star s.post frame }
+    in
+    match s with
+    | C_ST s -> C_ST (add_frame_s s)
+    | C_STAtomic inames s -> C_STAtomic inames (add_frame_s s)
+    | C_STGhost inames s -> C_STGhost inames (add_frame_s s)
 
 //
 // TODO: there is a observability flag upcoming in the underlying steel framework
 //       the bind will then also allow for (statomic unobservable, statomic observable)
 //       and the symmetric one
 //
-let bind_comp_compatible (c1 c2:pure_comp_st) : prop =
-  match c1, c2 with
-  | C_STGhost inames1 _, C_STGhost inames2 _ -> inames1 == inames2
-  | C_ST _, C_ST _ -> True
-  | _, _ -> False
+let bind_comp_compatible (c1 c2:comp_st)
+  : prop
+  = match c1, c2 with
+    | C_STGhost inames1 _, C_STGhost inames2 _ -> inames1 == inames2
+    | C_ST _, C_ST _ -> True
+    | _, _ -> False
 
-let bind_comp_pre (x:var) (c1 c2:pure_comp_st) : prop =
-  open_term (comp_post c1) x == comp_pre c2 /\
-  (~ (x `Set.mem` freevars (comp_post c2))) /\  //x doesn't escape in the result type
-  bind_comp_compatible c1 c2
+let bind_comp_pre (x:var) (c1 c2:comp_st)
+  : prop
+  = open_term (comp_post c1) x == comp_pre c2 /\
+    (~ (x `Set.mem` freevars (comp_post c2))) /\  //x doesn't escape in the result type
+    bind_comp_compatible c1 c2
 
-let bind_comp_out (c1:pure_comp_st) (c2:pure_comp_st{bind_comp_compatible c1 c2})
-  : pure_comp_st =
-  let s = {u=comp_u c2; res=comp_res c2; pre=comp_pre c1; post=comp_post c2} in
-  match c1, c2 with
-  | C_STGhost inames _, C_STGhost _ _ -> C_STGhost inames s
-  | C_ST _, C_ST _ -> C_ST s
+let bind_comp_out (c1:comp_st) (c2:comp_st{bind_comp_compatible c1 c2})
+  : comp_st
+  = let s = {u=comp_u c2; res=comp_res c2; pre=comp_pre c1; post=comp_post c2} in
+    match c1, c2 with
+    | C_STGhost inames _, C_STGhost _ _ -> C_STGhost inames s
+    | C_ST _, C_ST _ -> C_ST s
 
-let bind_comp_ghost_l_compatible (c1 c2:pure_comp_st) : prop =
-  match c1, c2 with
-  | C_STGhost inames1 _, C_STAtomic inames2 _ -> inames1 == inames2
-  | _, _ -> False
+let bind_comp_ghost_l_compatible (c1 c2:comp_st)
+  : prop
+  = match c1, c2 with
+    | C_STGhost inames1 _, C_STAtomic inames2 _ -> inames1 == inames2
+    | _, _ -> False
 
-let bind_comp_ghost_l_pre (x:var) (c1 c2:pure_comp_st) : prop =
-  open_term (comp_post c1) x == comp_pre c2 /\
-  (~ (x `Set.mem` freevars (comp_post c2))) /\  //x doesn't escape in the result type
-  bind_comp_ghost_l_compatible c1 c2
+let bind_comp_ghost_l_pre (x:var) (c1 c2:comp_st)
+  : prop
+  = open_term (comp_post c1) x == comp_pre c2 /\
+    (~ (x `Set.mem` freevars (comp_post c2))) /\  //x doesn't escape in the result type
+    bind_comp_ghost_l_compatible c1 c2
 
-let bind_comp_ghost_l_out (c1:pure_comp_st) (c2:pure_comp_st{bind_comp_ghost_l_compatible c1 c2})
-  : pure_comp_st =
-  let s = {u=comp_u c2; res=comp_res c2; pre=comp_pre c1; post=comp_post c2} in
-  match c1, c2 with
-  | C_STGhost inames _, C_STAtomic _ _ -> C_STAtomic inames s
-
-let bind_comp_ghost_r_compatible (c1 c2:pure_comp_st) : prop =
-  match c1, c2 with
-  | C_STAtomic inames1 _, C_STGhost inames2 _ -> inames1 == inames2
-  | _, _ -> False
-
-let bind_comp_ghost_r_pre (x:var) (c1 c2:pure_comp_st) : prop =
-  open_term (comp_post c1) x == comp_pre c2 /\
-  (~ (x `Set.mem` freevars (comp_post c2))) /\  //x doesn't escape in the result type
-  bind_comp_ghost_r_compatible c1 c2
-
-let bind_comp_ghost_r_out (c1:pure_comp_st) (c2:pure_comp_st{bind_comp_ghost_r_compatible c1 c2})
-  : pure_comp_st =
-  let s = {u=comp_u c2; res=comp_res c2; pre=comp_pre c1; post=comp_post c2} in
-  match c1, c2 with
-  | C_STAtomic inames _, C_STGhost _ _ -> C_STAtomic inames s
-
-let st_equiv_pre (c1 c2:pure_comp_st) : prop =
-  comp_u c1 == comp_u c2 /\ comp_res c1 == comp_res c2 /\
-  (match c1, c2 with
-   | C_ST _, C_ST _ -> True
-   | C_STAtomic inames1 _, C_STAtomic inames2 _ ->
-     inames1 == inames2
-   | C_STGhost inames1 _, C_STGhost inames2 _ ->
-     inames1 == inames2
-   | _, _ -> False)
-
-let non_informative_witness_t (u:universe) (t:pure_term) : pure_term =
-  Tm_PureApp (Tm_UInst non_informative_witness_lid [u])
-             None
-             t
-
-let elim_exists_post (u:universe) (t:pure_term) (p:pure_term)
-  (x:var) : pure_term =
+let bind_comp_ghost_l_out (c1:comp_st) (c2:comp_st{bind_comp_ghost_l_compatible c1 c2})
+  : comp_st
+  = let s = {u=comp_u c2; res=comp_res c2; pre=comp_pre c1; post=comp_post c2} in
+    match c1, c2 with
+    | C_STGhost inames _, C_STAtomic _ _ -> C_STAtomic inames s
   
-  let x_tm = Tm_Var {nm_index=x;nm_ppname=RT.pp_name_default} in
-  let p = open_term' p (mk_reveal u t x_tm) 0 in
-  close_term p x
+let bind_comp_ghost_r_compatible (c1 c2:comp_st)
+  : prop
+  = match c1, c2 with
+    | C_STAtomic inames1 _, C_STGhost inames2 _ -> inames1 == inames2
+    | _, _ -> False
 
-let comp_elim_exists (u:universe) (t:pure_term) (p:pure_term) (x:var)
-  : pure_comp =
+let bind_comp_ghost_r_pre (x:var) (c1 c2:comp_st)
+  : prop
+  = open_term (comp_post c1) x == comp_pre c2 /\
+    (~ (x `Set.mem` freevars (comp_post c2))) /\  //x doesn't escape in the result type
+    bind_comp_ghost_r_compatible c1 c2
 
-  C_STGhost Tm_EmpInames {
-    u=u;
-    res=mk_erased u t;
-    pre=Tm_ExistsSL u t p;
-    post=elim_exists_post u t p x
-  }
+let bind_comp_ghost_r_out (c1:comp_st) (c2:comp_st{bind_comp_ghost_r_compatible c1 c2})
+  : comp_st
+  = let s = {u=comp_u c2; res=comp_res c2; pre=comp_pre c1; post=comp_post c2} in
+    match c1, c2 with
+    | C_STAtomic inames _, C_STGhost _ _ -> C_STAtomic inames s
 
-let comp_intro_exists (u:universe) (t:pure_term) (p:pure_term) (e:pure_term)
-  : pure_comp =
+let st_equiv_pre (c1 c2:comp_st)
+  : prop
+  = comp_u c1 == comp_u c2 /\ comp_res c1 == comp_res c2 /\
+    (match c1, c2 with
+    | C_ST _, C_ST _ -> True
+    | C_STAtomic inames1 _, C_STAtomic inames2 _ ->
+      inames1 == inames2
+    | C_STGhost inames1 _, C_STGhost inames2 _ ->
+      inames1 == inames2
+    | _, _ -> False)
 
-  assert (is_pure_term (open_term' p e 0));
-  C_STGhost Tm_EmpInames {
-    u=U_zero;
-    res=tm_unit;
-    pre=open_term' p e 0;
-    post=Tm_ExistsSL u t p
-  }
+let non_informative_witness_t (u:universe) (t:term)
+  : term
+  = Tm_PureApp (Tm_UInst non_informative_witness_lid [u])
+               None
+               t
 
-let comp_while_cond (inv:pure_term) : pure_comp = C_ST {
-  u=U_zero;
-  res=tm_bool;
-  pre=Tm_ExistsSL U_zero tm_bool inv;
-  post=inv
-}
+let elim_exists_post (u:universe) (t:term) (p:term) (x:var)
+  : term
+  = let x_tm = Tm_Var {nm_index=x;nm_ppname=RT.pp_name_default} in
+    let p = open_term' p (mk_reveal u t x_tm) 0 in
+    close_term p x
 
-let comp_while_body (inv:pure_term) : pure_comp =
-  assert (is_pure_term (open_term' inv tm_true 0));
-  C_ST {
-    u=U_zero;
-    res=tm_unit;
-    pre=open_term' inv tm_true 0;
-    post=Tm_ExistsSL U_zero tm_bool inv
-}
+let comp_elim_exists (u:universe) (t:term) (p:term) (x:var)
+  : comp
+  = C_STGhost Tm_EmpInames 
+              {
+                u=u;
+                res=mk_erased u t;
+                pre=Tm_ExistsSL u t p;
+                post=elim_exists_post u t p x
+              }
 
-let comp_while (inv:pure_term) : pure_comp =
-  assert (is_pure_term (open_term' inv tm_false 0));
-  C_ST {
-    u=U_zero;
-    res=tm_unit;
-    pre=Tm_ExistsSL U_zero tm_bool inv;
-    post=open_term' inv tm_false 0
-}
+let comp_intro_exists (u:universe) (t:term) (p:term) (e:term)
+  : comp
+  = C_STGhost Tm_EmpInames
+              {
+                u=U_zero;
+                res=tm_unit;
+                pre=open_term' p e 0;
+                post=Tm_ExistsSL u t p
+              }
+
+let comp_while_cond (inv:term)
+  : comp
+  = C_ST {
+           u=U_zero;
+           res=tm_bool;
+           pre=Tm_ExistsSL U_zero tm_bool inv;
+           post=inv
+         }
+
+let comp_while_body (inv:term)
+  : comp
+  = C_ST {
+           u=U_zero;
+           res=tm_unit;
+           pre=open_term' inv tm_true 0;
+           post=Tm_ExistsSL U_zero tm_bool inv
+         }
+
+let comp_while (inv:term)
+  : comp
+  = C_ST {
+           u=U_zero;
+           res=tm_unit;
+           pre=Tm_ExistsSL U_zero tm_bool inv;
+           post=open_term' inv tm_false 0
+         }
 
 [@@erasable]
 noeq
 type my_erased (a:Type) = | E of a
 
-#push-options "--z3rlimit_factor 2"
+
+let typing (f:RT.fstar_top_env) (g:env) (e:term) (t:term) =
+    RT.typing (extend_env_l f g) (elab_term e) (elab_term t)
+
+let tot_typing (f:RT.fstar_top_env) (g:env) (e:term) (t:term) =
+    my_erased (typing f g e t)
+
+let universe_of (f:RT.fstar_top_env) (g:env) (t:term) (u:universe) =
+    tot_typing f g t (Tm_Type u)
+
 [@@ no_auto_projectors]
 noeq
-type src_typing (f:RT.fstar_top_env) : env -> term -> pure_comp -> Type =
-  | T_Tot: 
-      g:env ->
-      e:pure_term ->
-      ty:pure_term ->
-      RT.typing (extend_env_l f g) (elab_pure e) (elab_pure ty) ->
-      src_typing f g e (C_Tot ty)
-
-  | T_Abs: 
-      g:env ->
-      ppname:ppname ->
-      x:var { None? (lookup g x) } ->
-      q:option qualifier ->
-      ty:pure_term ->
-      u:universe ->
-      body:term {~ (x `Set.mem` freevars body) } ->
-      c:pure_comp ->
-      tot_typing f g ty (Tm_Type u) ->
-      src_typing f ((x, Inl ty)::g) (open_term body x) c ->
-      src_typing f g (Tm_Abs {binder_ty=ty;binder_ppname=ppname} q None body None)
-                     (C_Tot (Tm_Arrow {binder_ty=ty;binder_ppname=ppname} q (close_pure_comp c x)))
-  
-  | T_STApp :
-      g:env ->
-      head:term ->
-      ppname:ppname ->
-      formal:pure_term ->
-      q:option qualifier ->
-      res:pure_comp {stateful_comp res} ->
-      arg:pure_term ->
-      src_typing f g head (C_Tot (Tm_Arrow {binder_ty=formal;binder_ppname=ppname} q res)) ->
-      tot_typing f g arg formal ->
-      src_typing f g (Tm_STApp head q arg) (open_comp_with res arg)
-
-  | T_Return:
-      g:env ->
-      e:pure_term -> 
-      t:pure_term -> 
-      u:universe ->
-      tot_typing f g e t ->
-      universe_of f g t u ->
-      src_typing f g e (return_comp u t e)
-
-  | T_ReturnNoEq:
-      g:env ->
-      e:term -> 
-      t:pure_term -> 
-      u:universe ->
-      src_typing f g e (C_Tot t) ->
-      universe_of f g t u ->
-      src_typing f g e (return_comp_noeq u t)
-
-  | T_Lift:
-      g:env ->
-      e:term ->
-      c1:pure_comp_st ->
-      c2:pure_comp_st ->
-      src_typing f g e c1 ->
-      lift_comp f g c1 c2 ->
-      src_typing f g e c2
-
-  | T_Bind:
-      g:env ->
-      e1:term ->
-      e2:term ->
-      c1:pure_comp_st ->
-      c2:pure_comp_st ->
-      x:var { None? (lookup g x)  /\ ~(x `Set.mem` freevars e2) } ->
-      c:pure_comp ->
-      src_typing f g e1 c1 ->
-      tot_typing f g (comp_res c1) (Tm_Type (comp_u c1)) -> //type-correctness; would be nice to derive it instead      
-      src_typing f ((x, Inl (comp_res c1))::g) (open_term e2 x) c2 ->
-      bind_comp f g x c1 c2 c ->
-      src_typing f g (Tm_Bind e1 e2) c
-
-  | T_If:
-      g:env ->
-      b:pure_term -> 
-      e1:term ->
-      e2:term ->
-      c:pure_comp_st ->
-      uc:universe ->
-      (* This is a little weird, we introduce a name hyp in the environment, 
-         but the branches are not allowed to use it (except perhaps in a silent way for proofs).
-         Maybe more natural to have one free var in e1,e2 and to open it with hyp?
-         But that's also a change to Refl.Typing
-       *)
-      hyp:var { None? (lookup g hyp) /\
-               ~(hyp `Set.mem` (freevars e1 `Set.union` freevars e2))
-              } ->
-      tot_typing f g b tm_bool ->
-      src_typing f ((hyp, Inl (mk_eq2 U_zero tm_bool b tm_true)) :: g) e1 c ->
-      src_typing f ((hyp, Inl (mk_eq2 U_zero tm_bool b tm_false)) :: g) e2 c ->
-      my_erased (comp_typing f g c uc) ->
-      src_typing f g (Tm_If b e1 e2 None) c
-
-  | T_Frame:
-      g:env ->
-      e:term ->
-      c:pure_comp_st ->
-      frame:pure_term ->
-      tot_typing f g frame Tm_VProp ->
-      src_typing f g e c ->
-      src_typing f g e (add_frame c frame)
-
-  | T_Equiv:
-      g:env ->
-      e:term ->
-      c:pure_comp ->
-      c':pure_comp ->      
-      src_typing f g e c ->
-      st_equiv f g c c' ->
-      src_typing f g e c'
-
-  | T_ElimExists:
-      g:env ->
-      u:universe ->
-      t:pure_term ->
-      p:pure_term ->
-      x:var { None? (lookup g x) } ->
-      tot_typing f g t (Tm_Type u) ->
-      tot_typing f g (Tm_ExistsSL u t p) Tm_VProp ->
-      src_typing f g (Tm_ElimExists (Tm_ExistsSL u t p))
-                     (comp_elim_exists u t p x)
-
-  | T_IntroExists:
-      g:env ->
-      u:universe ->
-      t:pure_term ->
-      p:pure_term ->
-      e:pure_term ->
-      tot_typing f g t (Tm_Type u) ->
-      tot_typing f g (Tm_ExistsSL u t p) Tm_VProp ->
-      tot_typing f g e t ->
-      src_typing f g (Tm_IntroExists e (Tm_ExistsSL u t p))
-                     (comp_intro_exists u t p e)
-
-  | T_While:
-      g:env ->
-      inv:pure_term ->
-      cond:term ->
-      body:term ->
-      tot_typing f g (Tm_ExistsSL U_zero tm_bool inv) Tm_VProp ->
-      src_typing f g cond (comp_while_cond inv) ->
-      src_typing f g body (comp_while_body inv) ->
-      src_typing f g (Tm_While inv cond body) (comp_while inv)
-      
-
-and tot_typing (f:RT.fstar_top_env) (g:env) (e:term) (t:pure_term) =
-  my_erased (src_typing f g e (C_Tot t))
-
-and universe_of (f:RT.fstar_top_env) (g:env) (t:term) (u:universe) =
-  tot_typing f g t (Tm_Type u)
-
-and bind_comp (f:RT.fstar_top_env) : env -> var -> pure_comp -> pure_comp -> pure_comp -> Type =
-  | Bind_comp :  // (C_ST and C_ST) or (C_STGhost and C_STGhost)
-      g:env ->
-      x:var { None? (lookup g x) } ->
-      c1:pure_comp_st ->
-      c2:pure_comp_st {bind_comp_pre x c1 c2} ->
-      universe_of f g (comp_res c2) (comp_u c2) ->
-      //or in the result post; free var check isn't enough; we need typability
-      y:var { None? (lookup g y) /\ ~(y `Set.mem` freevars (comp_post c2)) } ->      
-      tot_typing f ((y, Inl (comp_res c2)) :: g) (open_term (comp_post c2) y) Tm_VProp ->
-      bind_comp f g x c1 c2 (bind_comp_out c1 c2)
-
-  | Bind_comp_ghost_l :  // (C_STGhost and C_STAtomic)
-      g:env ->
-      x:var { None? (lookup g x) } ->
-      c1:pure_comp_st ->
-      c2:pure_comp_st {bind_comp_ghost_l_pre x c1 c2} ->
-      non_informative_c1:(w:pure_term & src_typing f g w (C_Tot (non_informative_witness_t (comp_u c1) (comp_res c1)))) ->
-      universe_of f g (comp_res c2) (comp_u c2) ->
-      //or in the result post; free var check isn't enough; we need typability
-      y:var { None? (lookup g y) /\ ~(y `Set.mem` freevars (comp_post c2)) } ->
-      tot_typing f ((y, Inl (comp_res c2)) :: g) (open_term (comp_post c2) y) Tm_VProp ->
-      bind_comp f g x c1 c2 (bind_comp_ghost_l_out c1 c2)
-
-  | Bind_comp_ghost_r :  // (C_STAtomic and C_STGhost)
-      g:env ->
-      x:var { None? (lookup g x) } ->
-      c1:pure_comp_st ->
-      c2:pure_comp_st {bind_comp_ghost_r_pre x c1 c2} ->
-      non_informative_c2:(w:pure_term & src_typing f g w (C_Tot (non_informative_witness_t (comp_u c2) (comp_res c2)))) ->
-      universe_of f g (comp_res c2) (comp_u c2) ->
-      //or in the result post; free var check isn't enough; we need typability
-      y:var { None? (lookup g y) /\ ~(y `Set.mem` freevars (comp_post c2)) } ->
-      tot_typing f ((y, Inl (comp_res c2)) :: g) (open_term (comp_post c2) y) Tm_VProp ->
-      bind_comp f g x c1 c2 (bind_comp_ghost_r_out c1 c2)
-
-and lift_comp (f:RT.fstar_top_env) : env -> pure_comp -> pure_comp -> Type =
-  | Lift_STAtomic_ST :
-      g:env ->
-      c:pure_comp_st{C_STAtomic? c /\ comp_inames c == Tm_EmpInames} ->
-      lift_comp f g c (C_ST (st_comp_of_comp c))
-
-  | Lift_STGhost_STAtomic :
-      g:env ->
-      c:pure_comp_st{C_STGhost? c} ->
-      non_informative_c:(w:pure_term & src_typing f g w (C_Tot (non_informative_witness_t (comp_u c) (comp_res c)))) ->
-      lift_comp f g c (C_STAtomic (comp_inames c) (st_comp_of_comp c))
-
-and st_equiv (f:RT.fstar_top_env) : env -> pure_comp -> pure_comp -> Type =
+type st_equiv (f:RT.fstar_top_env) : env -> comp -> comp -> Type =
   | ST_VPropEquiv :
       g:env ->
-      c1:pure_comp_st ->
-      c2:pure_comp_st { st_equiv_pre c1 c2 } -> 
+      c1:comp_st ->
+      c2:comp_st { st_equiv_pre c1 c2 } -> 
       x:var { None? (lookup g x) /\ ~(x `Set.mem` freevars (comp_post c1)) /\ ~(x `Set.mem` freevars (comp_post c2)) } ->
       tot_typing f g (comp_pre c1) Tm_VProp ->
       tot_typing f g (comp_res c1) (Tm_Type (comp_u c1)) ->
@@ -581,10 +394,24 @@ and st_equiv (f:RT.fstar_top_env) : env -> pure_comp -> pure_comp -> Type =
                     (open_term (comp_post c2) x) ->      
       st_equiv f g c1 c2
 
-and comp_typing (f:RT.fstar_top_env) : env -> comp -> universe -> Type =
+[@@ no_auto_projectors]
+noeq
+type st_comp_typing (f:RT.fstar_top_env) : env -> st_comp -> Type =
+  | STC:
+      g:env -> 
+      st:st_comp ->
+      x:var { None? (lookup g x) /\ ~(x `Set.mem` freevars st.post) } ->
+      universe_of f g st.res st.u ->
+      tot_typing f g st.pre Tm_VProp ->
+      tot_typing f ((x, Inl st.res)::g) (open_term st.post x) Tm_VProp ->
+      st_comp_typing f g st
+
+[@@ no_auto_projectors]
+noeq
+type comp_typing (f:RT.fstar_top_env) : env -> comp -> universe -> Type =
   | CT_Tot :
       g:env ->
-      t:pure_term ->
+      t:term ->
       u:universe ->
       universe_of f g t u ->
       comp_typing f g (C_Tot t) u
@@ -597,7 +424,7 @@ and comp_typing (f:RT.fstar_top_env) : env -> comp -> universe -> Type =
 
   | CT_STAtomic :
       g:env -> 
-      inames:pure_term ->
+      inames:term ->
       st:st_comp -> 
       tot_typing f g inames Tm_Inames ->
       st_comp_typing f g st ->
@@ -605,23 +432,216 @@ and comp_typing (f:RT.fstar_top_env) : env -> comp -> universe -> Type =
 
   | CT_STGhost :
       g:env -> 
-      inames:pure_term ->
+      inames:term ->
       st:st_comp -> 
       tot_typing f g inames Tm_Inames ->      
       st_comp_typing f g st ->
       comp_typing f g (C_STGhost inames st) st.u
 
-and st_comp_typing (f:RT.fstar_top_env) : env -> st_comp -> Type =
-  | STC:
-      g:env -> 
-      st:st_comp { is_pure_st_comp st } -> 
-      x:var { None? (lookup g x) /\ ~(x `Set.mem` freevars st.post) } ->
-      universe_of f g st.res st.u ->
-      tot_typing f g st.pre Tm_VProp ->
-      tot_typing f ((x, Inl st.res)::g) (open_term st.post x) Tm_VProp ->
-      st_comp_typing f g st
-      
-#pop-options
+let non_informative (f:RT.fstar_top_env) (g:env) (c:comp_st) =
+    w:term & tot_typing f g w (non_informative_witness_t (comp_u c) (comp_res c))
+     
+[@@ no_auto_projectors]
+noeq
+type bind_comp (f:RT.fstar_top_env) : env -> var -> comp -> comp -> comp -> Type =
+  | Bind_comp :  // (C_ST and C_ST) or (C_STGhost and C_STGhost)
+      g:env ->
+      x:var { None? (lookup g x) } ->
+      c1:comp_st ->
+      c2:comp_st {bind_comp_pre x c1 c2} ->
+      universe_of f g (comp_res c2) (comp_u c2) ->
+      //or in the result post; free var check isn't enough; we need typability
+      y:var { None? (lookup g y) /\ ~(y `Set.mem` freevars (comp_post c2)) } ->      
+      tot_typing f ((y, Inl (comp_res c2)) :: g) (open_term (comp_post c2) y) Tm_VProp ->
+      bind_comp f g x c1 c2 (bind_comp_out c1 c2)
+
+  | Bind_comp_ghost_l :  // (C_STGhost and C_STAtomic)
+      g:env ->
+      x:var { None? (lookup g x) } ->
+      c1:comp_st ->
+      c2:comp_st {bind_comp_ghost_l_pre x c1 c2} ->
+      non_informative_c1:non_informative f g c1 ->
+      universe_of f g (comp_res c2) (comp_u c2) ->
+      //or in the result post; free var check isn't enough; we need typability
+      y:var { None? (lookup g y) /\ ~(y `Set.mem` freevars (comp_post c2)) } ->
+      tot_typing f ((y, Inl (comp_res c2)) :: g) (open_term (comp_post c2) y) Tm_VProp ->
+      bind_comp f g x c1 c2 (bind_comp_ghost_l_out c1 c2)
+
+  | Bind_comp_ghost_r :  // (C_STAtomic and C_STGhost)
+      g:env ->
+      x:var { None? (lookup g x) } ->
+      c1:comp_st ->
+      c2:comp_st {bind_comp_ghost_r_pre x c1 c2} ->
+      non_informative_c2:non_informative f g c2 ->
+      universe_of f g (comp_res c2) (comp_u c2) ->
+      //or in the result post; free var check isn't enough; we need typability
+      y:var { None? (lookup g y) /\ ~(y `Set.mem` freevars (comp_post c2)) } ->
+      tot_typing f ((y, Inl (comp_res c2)) :: g) (open_term (comp_post c2) y) Tm_VProp ->
+      bind_comp f g x c1 c2 (bind_comp_ghost_r_out c1 c2)
+
+[@@ no_auto_projectors]
+noeq
+type lift_comp (f:RT.fstar_top_env) : env -> comp -> comp -> Type =
+  | Lift_STAtomic_ST :
+      g:env ->
+      c:comp_st{C_STAtomic? c /\ comp_inames c == Tm_EmpInames} ->
+      lift_comp f g c (C_ST (st_comp_of_comp c))
+
+  | Lift_STGhost_STAtomic :
+      g:env ->
+      c:comp_st{C_STGhost? c} ->
+      non_informative_c:non_informative f g c ->
+      lift_comp f g c (C_STAtomic (comp_inames c) (st_comp_of_comp c))
+
+let as_binder t = { binder_ty = t; binder_ppname = RT.pp_name_default }
+
+[@@ no_auto_projectors]
+noeq
+type st_typing (f:RT.fstar_top_env) : env -> st_term -> comp -> Type =
+  | T_Tot:
+      g:env ->
+      e:term ->
+      ty:term ->
+      tot_typing f g e ty ->
+      st_typing f g (Tm_Return e) (C_Tot ty)
+
+  | T_Abs: 
+      g:env ->
+      x:var { None? (lookup g x) } ->
+      q:option qualifier ->
+      ty:term ->
+      u:universe ->
+      body:st_term {~ (x `Set.mem` freevars_st body) } ->
+      c:comp ->
+      tot_typing f g ty (Tm_Type u) ->
+      st_typing f ((x, Inl ty)::g) (open_term_st body x) c ->
+      st_typing f g (Tm_Abs (as_binder ty) q None body None)
+                    (C_Tot (Tm_Arrow (as_binder ty) q (close_comp c x)))
+  
+  | T_STApp :
+      g:env ->
+      head:st_term ->
+      ty:term ->
+      q:option qualifier ->
+      res:comp_st ->
+      arg:term ->
+      st_typing f g head (C_Tot (Tm_Arrow (as_binder ty) q res)) ->
+      tot_typing f g arg ty ->
+      st_typing f g (Tm_STApp head q arg) (open_comp_with res arg)
+
+  | T_Return:
+      g:env ->
+      e:term -> 
+      t:term -> 
+      u:universe ->
+      tot_typing f g e t ->
+      universe_of f g t u ->
+      st_typing f g (Tm_Return e) (return_comp u t e)
+
+  | T_ReturnNoEq:
+      g:env ->
+      e:st_term -> 
+      t:term -> 
+      u:universe ->
+      st_typing f g e (C_Tot t) ->
+      universe_of f g t u ->
+      st_typing f g e (return_comp_noeq u t)
+
+  | T_Lift:
+      g:env ->
+      e:st_term ->
+      c1:comp_st ->
+      c2:comp_st ->
+      st_typing f g e c1 ->
+      lift_comp f g c1 c2 ->
+      st_typing f g e c2
+
+  | T_Bind:
+      g:env ->
+      e1:st_term ->
+      e2:st_term ->
+      c1:comp_st ->
+      c2:comp_st ->
+      x:var { None? (lookup g x)  /\ ~(x `Set.mem` freevars_st e2) } ->
+      c:comp ->
+      st_typing f g e1 c1 ->
+      tot_typing f g (comp_res c1) (Tm_Type (comp_u c1)) -> //type-correctness; would be nice to derive it instead      
+      st_typing f ((x, Inl (comp_res c1))::g) (open_term_st e2 x) c2 ->
+      bind_comp f g x c1 c2 c ->
+      st_typing f g (Tm_Bind e1 e2) c
+
+  | T_If:
+      g:env ->
+      b:term -> 
+      e1:st_term ->
+      e2:st_term ->
+      c:comp_st ->
+      uc:universe ->
+      (* This is a little weird, we introduce a name hyp in the environment, 
+         but the branches are not allowed to use it (except perhaps in a silent way for proofs).
+         Maybe more natural to have one free var in e1,e2 and to open it with hyp?
+         But that's also a change to Refl.Typing
+       *)
+      hyp:var { None? (lookup g hyp) /\
+               ~(hyp `Set.mem` (freevars_st e1 `Set.union` freevars_st e2))
+              } ->
+      tot_typing f g b tm_bool ->
+      st_typing f ((hyp, Inl (mk_eq2 U_zero tm_bool b tm_true)) :: g) e1 c ->
+      st_typing f ((hyp, Inl (mk_eq2 U_zero tm_bool b tm_false)) :: g) e2 c ->
+      my_erased (comp_typing f g c uc) ->
+      st_typing f g (Tm_If b e1 e2 None) c
+
+  | T_Frame:
+      g:env ->
+      e:st_term ->
+      c:comp_st ->
+      frame:term ->
+      tot_typing f g frame Tm_VProp ->
+      st_typing f g e c ->
+      st_typing f g e (add_frame c frame)
+
+  | T_Equiv:
+      g:env ->
+      e:st_term ->
+      c:comp ->
+      c':comp ->      
+      st_typing f g e c ->
+      st_equiv f g c c' ->
+      st_typing f g e c'
+
+  | T_ElimExists:
+      g:env ->
+      u:universe ->
+      t:term ->
+      p:term ->
+      x:var { None? (lookup g x) } ->
+      tot_typing f g t (Tm_Type u) ->
+      tot_typing f g (Tm_ExistsSL u t p) Tm_VProp ->
+      st_typing f g (Tm_ElimExists (Tm_ExistsSL u t p))
+                    (comp_elim_exists u t p x)
+
+  | T_IntroExists:
+      g:env ->
+      u:universe ->
+      t:term ->
+      p:term ->
+      e:term ->
+      tot_typing f g t (Tm_Type u) ->
+      tot_typing f g (Tm_ExistsSL u t p) Tm_VProp ->
+      tot_typing f g e t ->
+      st_typing f g (Tm_IntroExists e (Tm_ExistsSL u t p))
+                    (comp_intro_exists u t p e)
+
+  | T_While:
+      g:env ->
+      inv:term ->
+      cond:st_term ->
+      body:st_term ->
+      tot_typing f g (Tm_ExistsSL U_zero tm_bool inv) Tm_VProp ->
+      st_typing f g cond (comp_while_cond inv) ->
+      st_typing f g body (comp_while_body inv) ->
+      st_typing f g (Tm_While inv cond body) (comp_while inv)
+
 
 (* this requires some metatheory on Refl.Typing
 
@@ -646,8 +666,9 @@ let star_typing_inversion (f:_) (g:_) (t0 t1:term) (d:tot_typing f g (Tm_Star t0
      tot_typing f g t1 Tm_VProp)
   = admit()
 
-let vprop_eq_typing_inversion (f:RT.fstar_top_env) g (t0 t1:pure_term)
-  (token:FTB.prop_validity_token (extend_env_l f g) (elab_pure (mk_vprop_eq t0 t1)))
+let vprop_eq_typing_inversion (f:RT.fstar_top_env) g (t0 t1:term)
+                              (token:FTB.prop_validity_token (extend_env_l f g)
+                                                             (elab_term (mk_vprop_eq t0 t1)))
   : (tot_typing f g t0 Tm_VProp &
      tot_typing f g t1 Tm_VProp)
   = admit ()
@@ -663,7 +684,7 @@ let emp_typing (#f:_) (#g:_)
   : tot_typing f g Tm_Emp Tm_VProp
   = admit()
 
-let rec vprop_equiv_typing (f:_) (g:_) (t0 t1:pure_term) (v:vprop_equiv f g t0 t1)
+let rec vprop_equiv_typing (f:_) (g:_) (t0 t1:term) (v:vprop_equiv f g t0 t1)
   : GTot ((tot_typing f g t0 Tm_VProp -> tot_typing f g t1 Tm_VProp) &
           (tot_typing f g t1 Tm_VProp -> tot_typing f g t0 Tm_VProp))
         (decreases v)
